Morph.v
@@ -17,6 +17,7 @@ Open Scope nat_scope.
 
 Inductive SSError : Set :=
   | ERegistersExhausted : nat -> SSError
+  | ENoValidSplitPosition : nat -> SSError
   | ECannotSplitSingleton2 : nat -> IntervalDesc -> nat -> SSError
   | ECannotSplitSingleton3 : nat -> SSError
   | ECannotSplitSingleton4 : nat -> SSError
